Prove useful lemmas about the extra state for blake2

code/hash/Hacl.Hash.Blake2.fst
@@ -115,8 +115,6 @@ let blake2_update_last_block_st (a : hash_alg{is_blake a}) =
         Spec.Blake2.blake2_update_last (to_blake_alg a) (v #U64 #SEC ev)
                                        (v input_len) (B.as_seq h0 input) (as_seq h0 s)))
 
-(* TODO: ajouter Spec.Blake2.blake2_update_last: *)
-
 noextract inline_for_extraction
 val mk_update_last: a:hash_alg{is_blake a} -> update_multi_st a ->
                     blake2_update_last_block_st a -> update_last_st a
@@ -152,6 +150,345 @@ let mk_update_last a update_multi blake2_update_last_block s ev prev_len input i
   ST.pop_frame ();
   u64 0
 #pop-options
+
+(*
+U128.uint64_to_uint128
+(*
+  u64 0
+
+  admit()
+
+
+let test (a:hash_alg{is_blake a})
+  (hash:words_state a)
+  (prevlen:nat{prevlen % block_length a = 0})
+  (input:bytes{S.length input + prevlen <= max_input_length a}): unit =
+  let h1 = Spec.Hash.Incremental.update_last_blake a hash prevlen input in
+  (**)
+  let blocks, last_block, rem = Spec.Hash.Incremental.last_split_blake a input in
+  let h' = Spec.Agile.Hash.update_multi a hash blocks in
+  let h_f = Spec.Blake2.blake2_update_block (to_blake_alg a) true (v (snd h' +. u64 rem)) last_block (fst h') in
+  (**)
+  assume(v #U64 #SEC (snd h') == Seq.length blocks);
+  assert(Seq.length input = Seq.length blocks + rem);
+  let input_rem = Seq.slice input (Seq.length blocks) (Seq.length input) in
+  let h2 = Spec.Blake2.blake2_update_last (to_blake_alg a) (Seq.length blocks) rem input_rem (fst h') in
+  assert(h_f == h2)
+
+  
+
+  calc (==) {
+    v rest_len % block_length a;
+    (==) { }
+    ((v input_len - v blocks_len) % pow2 64) % block_length a;
+    (==) {
+      assert_norm (block_length Blake2S == pow2 6);
+      assert_norm (block_length Blake2B == pow2 7);
+      FStar.Math.Lemmas.pow2_modulo_modulo_lemma_1 (v input_len - v blocks_len) 6 64;
+      FStar.Math.Lemmas.pow2_modulo_modulo_lemma_1 (v input_len - v blocks_len) 6 64
+      }
+    (v input_len - v blocks_len) % block_length a;
+    (==) { FStar.Math.Lemmas.lemma_mod_sub_distr (v input_len) (v blocks_len) (block_length a) }
+    v input_len % block_length a;
+  };
+
+  calc (==) {
+    (block_length a - (len_v a prev_len + v input_len) ) % block_length a;
+    (==) { FStar.Math.Lemmas.lemma_mod_sub_distr (block_length a - v input_len) (len_v a prev_len) (block_length a) }
+    (block_length a - v input_len) % block_length a;
+    (==) { FStar.Math.Lemmas.lemma_mod_sub_distr (block_length a) (v input_len) (block_length a) }
+    (block_length a - (v input_len % block_length a)) % block_length a;
+    (==) { }
+    (block_length a - (v rest_len % block_length a)) % block_length a;
+    (==) { FStar.Math.Lemmas.lemma_mod_sub_distr (block_length a) (v rest_len) (block_length a) }
+    (block_length a - v rest_len) % block_length a;
+  };
+
+  (* The rest that doesn't make up a complete block *)
+  assume(rest_len <> 0ul);
+  let rest = B.sub input blocks_len rest_len in
+
+  let pad_len = U32.(block_len a -^ rest_len) in
+
+  let tmp = B.alloca (Lib.IntTypes.u8 0) (block_len a) in
+  let tmp_rest = B.sub tmp 0ul rest_len in
+  let tmp_pad = B.sub tmp rest_len pad_len in
+  B.blit rest 0ul tmp_rest 0ul rest_len;
+
+  calc (==) {
+    (block_length a - (len_v a prev_len + v input_len) ) % block_length a;
+    (==) { }
+    (block_length a - v rest_len) % block_length a;
+    (==) { FStar.Math.Lemmas.small_mod (block_length a - v rest_len) (block_length a) }
+    block_length a - v rest_len;
+    (==) { assert_norm (block_length a <= pow2 32); FStar.Math.Lemmas.small_mod (block_length a - v rest_len) (pow2 32) }
+    v pad_len;
+  };
+
+  let h2 = ST.get() in
+
+  calc (==) {
+    B.as_seq h0 blocks `Seq.append` B.as_seq h2 tmp;
+    (==) { assert (Seq.equal (B.as_seq h2 tmp) (B.as_seq h2 tmp_rest `Seq.append` B.as_seq h2 tmp_pad)) }
+    B.as_seq h0 blocks `Seq.append` (B.as_seq h2 tmp_rest `Seq.append` B.as_seq h2 tmp_pad);
+    (==) { Seq.append_assoc (B.as_seq h0 blocks) (B.as_seq h2 tmp_rest) (B.as_seq h2 tmp_pad) }
+    (B.as_seq h0 blocks `Seq.append` B.as_seq h2 tmp_rest) `Seq.append` B.as_seq h2 tmp_pad;
+    (==) { assert (S.equal (B.as_seq h0 input) (S.append (B.as_seq h0 blocks) (B.as_seq h2 tmp_rest))) }
+    B.as_seq h0 input `Seq.append` B.as_seq h2 tmp_pad;
+    (==) { assert (B.as_seq h2 tmp_pad `S.equal` Spec.Hash.PadFinish.pad a (len_v a prev_len + v input_len)) }
+    B.as_seq h0 input `Seq.append` Spec.Hash.PadFinish.pad a (len_v a prev_len + v input_len);
+  };
+    
+  assume(B.as_seq h2 tmp `S.equal`
+    Spec.Blake2.get_last_padded_block (to_blake_alg a) (B.as_seq h0 input) (U32.v rest_len));
+
+  let ev_f = update_multi s ev' tmp 1ul in
+
+  Spec.Hash.Lemmas.update_multi_update a (as_seq h2 s, ev') (B.as_seq h2 tmp);
+
+  let h3 = ST.get() in
+
+//  assume(as_seq h3 s ==
+//    Spec.Agile.Hash.update_multi a (U32.v input_len)
+//                                 (B.as_seq h2 tmp) (as_seq h2 s));
+
+//  assert(as_seq h3 s ==
+//    Spec.Blake2.blake2_update_block (to_blake_alg a) true (Lib.IntTypes.v #U64 #SEC ev')
+//                                    (B.as_seq h2 tmp) (as_seq h2 s));
+  admit()
+
+extra_state
+
+  Spec.Hash.Lemmas.update_multi_associative a (as_seq h0 s, ev) (B.as_seq h0 blocks)
+                                            (B.as_seq h2 tmp);
+
+  ST.pop_frame();
+  ev_f
+  
+(****)
+
+  assume(rest_len == 0ul);
+  assert (Spec.Hash.PadFinish.pad a (len_v a prev_len + v input_len) `Seq.equal` Seq.empty);
+  assert (S.equal
+   (B.as_seq h0 input `Seq.append` (Spec.Hash.PadFinish.pad a (len_v a prev_len + v input_len)))
+   (B.as_seq h1 blocks));
+  ST.pop_frame();
+  ev'
+
+
+  assume(rest_len <> 0ul);
+  let rest = B.sub input blocks_len rest_len in
+
+  let pad_len = U32.(block_len a -^ rest_len) in
+
+  let tmp = B.alloca (Lib.IntTypes.u8 0) (block_len a) in
+  let tmp_rest = B.sub tmp 0ul rest_len in
+  let tmp_pad = B.sub tmp rest_len pad_len in
+  B.blit rest 0ul tmp_rest 0ul rest_len;
+
+  calc (==) {
+    (block_length a - (len_v a prev_len + v input_len) ) % block_length a;
+    (==) { }
+    (block_length a - v rest_len) % block_length a;
+    (==) { FStar.Math.Lemmas.small_mod (block_length a - v rest_len) (block_length a) }
+    block_length a - v rest_len;
+    (==) { assert_norm (block_length a <= pow2 32); FStar.Math.Lemmas.small_mod (block_length a - v rest_len) (pow2 32) }
+    v pad_len;
+  };
+
+  let h2 = ST.get() in
+
+  calc (==) {
+    B.as_seq h0 blocks `Seq.append` B.as_seq h2 tmp;
+    (==) { assert (Seq.equal (B.as_seq h2 tmp) (B.as_seq h2 tmp_rest `Seq.append` B.as_seq h2 tmp_pad)) }
+    B.as_seq h0 blocks `Seq.append` (B.as_seq h2 tmp_rest `Seq.append` B.as_seq h2 tmp_pad);
+    (==) { Seq.append_assoc (B.as_seq h0 blocks) (B.as_seq h2 tmp_rest) (B.as_seq h2 tmp_pad) }
+    (B.as_seq h0 blocks `Seq.append` B.as_seq h2 tmp_rest) `Seq.append` B.as_seq h2 tmp_pad;
+    (==) { assert (S.equal (B.as_seq h0 input) (S.append (B.as_seq h0 blocks) (B.as_seq h2 tmp_rest))) }
+    B.as_seq h0 input `Seq.append` B.as_seq h2 tmp_pad;
+    (==) { assert (B.as_seq h2 tmp_pad `S.equal` Spec.Hash.PadFinish.pad a (len_v a prev_len + v input_len)) }
+    B.as_seq h0 input `Seq.append` Spec.Hash.PadFinish.pad a (len_v a prev_len + v input_len);
+  };
+
+  let ev_f = update_multi s ev' tmp 1ul in
+
+  let h3 = ST.get() in
+
+  Spec.Hash.Lemmas.update_multi_associative a (as_seq h0 s, ev) (B.as_seq h0 blocks)
+                                            (B.as_seq h2 tmp);
+
+  ST.pop_frame();
+  ev_f
+
+  assume(rest_len == 0ul);
+  assert (Spec.Hash.PadFinish.pad a (len_v a prev_len + v input_len) `Seq.equal` Seq.empty);
+  assert (S.equal
+   (B.as_seq h0 input `Seq.append` (Spec.Hash.PadFinish.pad a (len_v a prev_len + v input_len)))
+   (B.as_seq h1 blocks));
+  ST.pop_frame();
+  ev'
+
+(******)
+  (* The rest that doesn't make up a complete block *)
+  if rest_len = 0ul then
+    (assert (Spec.Hash.PadFinish.pad a (len_v a prev_len + v input_len) `Seq.equal` Seq.empty);
+     assert (S.equal
+      (B.as_seq h0 input `Seq.append` (Spec.Hash.PadFinish.pad a (len_v a prev_len + v input_len)))
+      (B.as_seq h1 blocks));
+    ST.pop_frame();
+    ev'
+    )
+  else (
+    let rest = B.sub input blocks_len rest_len in
+
+
+    let pad_len = U32.(block_len a -^ rest_len) in
+
+    let tmp = B.alloca (Lib.IntTypes.u8 0) (block_len a) in
+    let tmp_rest = B.sub tmp 0ul rest_len in
+    let tmp_pad = B.sub tmp rest_len pad_len in
+    B.blit rest 0ul tmp_rest 0ul rest_len;
+
+    calc (==) {
+      (block_length a - (len_v a prev_len + v input_len) ) % block_length a;
+      (==) { }
+      (block_length a - v rest_len) % block_length a;
+      (==) { FStar.Math.Lemmas.small_mod (block_length a - v rest_len) (block_length a) }
+      block_length a - v rest_len;
+      (==) { assert_norm (block_length a <= pow2 32); FStar.Math.Lemmas.small_mod (block_length a - v rest_len) (pow2 32) }
+      v pad_len;
+    };
+
+    let h2 = ST.get() in
+
+    calc (==) {
+      B.as_seq h0 blocks `Seq.append` B.as_seq h2 tmp;
+      (==) { assert (Seq.equal (B.as_seq h2 tmp) (B.as_seq h2 tmp_rest `Seq.append` B.as_seq h2 tmp_pad)) }
+      B.as_seq h0 blocks `Seq.append` (B.as_seq h2 tmp_rest `Seq.append` B.as_seq h2 tmp_pad);
+      (==) { Seq.append_assoc (B.as_seq h0 blocks) (B.as_seq h2 tmp_rest) (B.as_seq h2 tmp_pad) }
+      (B.as_seq h0 blocks `Seq.append` B.as_seq h2 tmp_rest) `Seq.append` B.as_seq h2 tmp_pad;
+      (==) { assert (S.equal (B.as_seq h0 input) (S.append (B.as_seq h0 blocks) (B.as_seq h2 tmp_rest))) }
+      B.as_seq h0 input `Seq.append` B.as_seq h2 tmp_pad;
+      (==) { assert (B.as_seq h2 tmp_pad `S.equal` Spec.Hash.PadFinish.pad a (len_v a prev_len + v input_len)) }
+      B.as_seq h0 input `Seq.append` Spec.Hash.PadFinish.pad a (len_v a prev_len + v input_len);
+    };
+
+    let ev_f = update_multi s ev' tmp 1ul in
+
+    let h3 = ST.get() in
+
+    Spec.Hash.Lemmas.update_multi_associative a (as_seq h0 s, ev) (B.as_seq h0 blocks)
+                                              (B.as_seq h2 tmp);
+
+    ST.pop_frame();
+    ev_f
+  )
+#pop-options
+
+
+let mk_update_last a update_multi s ev prev_len input input_len =
+  ST.push_frame ();
+  let h0 = ST.get () in
+
+  (* Get a series of complete blocks. *)
+  let blocks_n = U32.(input_len /^ block_len a) in
+  let blocks_len = U32.(blocks_n *^ block_len a) in
+  assert (U32.v blocks_len % block_length a = 0);
+  let blocks = B.sub input 0ul blocks_len in
+
+  let ev' = update_multi s ev blocks blocks_n in
+
+  let h1 = ST.get () in
+
+  assert (S.equal (as_seq h1 s) (fst (Spec.Agile.Hash.update_multi a (as_seq h0 s, ev) (B.as_seq h0 blocks))));
+
+  let rest_len = U32.(input_len -^ blocks_len) in
+
+  calc (==) {
+    v rest_len % block_length a;
+    (==) { }
+    ((v input_len - v blocks_len) % pow2 64) % block_length a;
+    (==) {
+      assert_norm (block_length Blake2S == pow2 6);
+      assert_norm (block_length Blake2B == pow2 7);
+      FStar.Math.Lemmas.pow2_modulo_modulo_lemma_1 (v input_len - v blocks_len) 6 64;
+      FStar.Math.Lemmas.pow2_modulo_modulo_lemma_1 (v input_len - v blocks_len) 6 64
+      }
+    (v input_len - v blocks_len) % block_length a;
+    (==) { FStar.Math.Lemmas.lemma_mod_sub_distr (v input_len) (v blocks_len) (block_length a) }
+    v input_len % block_length a;
+  };
+
+  calc (==) {
+    (block_length a - (len_v a prev_len + v input_len) ) % block_length a;
+    (==) { FStar.Math.Lemmas.lemma_mod_sub_distr (block_length a - v input_len) (len_v a prev_len) (block_length a) }
+    (block_length a - v input_len) % block_length a;
+    (==) { FStar.Math.Lemmas.lemma_mod_sub_distr (block_length a) (v input_len) (block_length a) }
+    (block_length a - (v input_len % block_length a)) % block_length a;
+    (==) { }
+    (block_length a - (v rest_len % block_length a)) % block_length a;
+    (==) { FStar.Math.Lemmas.lemma_mod_sub_distr (block_length a) (v rest_len) (block_length a) }
+    (block_length a - v rest_len) % block_length a;
+  };
+
+  (* The rest that doesn't make up a complete block *)
+  if rest_len = 0ul then
+    (assert (Spec.Hash.PadFinish.pad a (len_v a prev_len + v input_len) `Seq.equal` Seq.empty);
+     assert (S.equal
+      (B.as_seq h0 input `Seq.append` (Spec.Hash.PadFinish.pad a (len_v a prev_len + v input_len)))
+      (B.as_seq h1 blocks));
+    ST.pop_frame();
+    admit();
+    ev'
+    )
+  else (
+    let rest = B.sub input blocks_len rest_len in
+
+
+    let pad_len = U32.(block_len a -^ rest_len) in
+
+    let tmp = B.alloca (Lib.IntTypes.u8 0) (block_len a) in
+    let tmp_rest = B.sub tmp 0ul rest_len in
+    let tmp_pad = B.sub tmp rest_len pad_len in
+    B.blit rest 0ul tmp_rest 0ul rest_len;
+
+    calc (==) {
+      (block_length a - (len_v a prev_len + v input_len) ) % block_length a;
+      (==) { }
+      (block_length a - v rest_len) % block_length a;
+      (==) { FStar.Math.Lemmas.small_mod (block_length a - v rest_len) (block_length a) }
+      block_length a - v rest_len;
+      (==) { assert_norm (block_length a <= pow2 32); FStar.Math.Lemmas.small_mod (block_length a - v rest_len) (pow2 32) }
+      v pad_len;
+    };
+
+    let h2 = ST.get() in
+
+    calc (==) {
+      B.as_seq h0 blocks `Seq.append` B.as_seq h2 tmp;
+      (==) { assert (Seq.equal (B.as_seq h2 tmp) (B.as_seq h2 tmp_rest `Seq.append` B.as_seq h2 tmp_pad)) }
+      B.as_seq h0 blocks `Seq.append` (B.as_seq h2 tmp_rest `Seq.append` B.as_seq h2 tmp_pad);
+      (==) { Seq.append_assoc (B.as_seq h0 blocks) (B.as_seq h2 tmp_rest) (B.as_seq h2 tmp_pad) }
+      (B.as_seq h0 blocks `Seq.append` B.as_seq h2 tmp_rest) `Seq.append` B.as_seq h2 tmp_pad;
+      (==) { assert (S.equal (B.as_seq h0 input) (S.append (B.as_seq h0 blocks) (B.as_seq h2 tmp_rest))) }
+      B.as_seq h0 input `Seq.append` B.as_seq h2 tmp_pad;
+      (==) { assert (B.as_seq h2 tmp_pad `S.equal` Spec.Hash.PadFinish.pad a (len_v a prev_len + v input_len)) }
+      B.as_seq h0 input `Seq.append` Spec.Hash.PadFinish.pad a (len_v a prev_len + v input_len);
+    };
+
+    let ev_f = update_multi s ev' tmp 1ul in
+
+    let h3 = ST.get() in
+
+    Spec.Hash.Lemmas.update_multi_associative a (as_seq h0 s, ev) (B.as_seq h0 blocks) (B.as_seq h2 tmp);
+
+    ST.pop_frame();
+    admit();
+    ev_f
+  );
+  admit()
+#pop-options
+*)
 
 let update_multi_blake2s: update_multi_st Blake2S =
   mk_update_multi Blake2S update_blake2s
