specs/Spec.Hash.Lemmas.fst
@@ -4,11 +4,45 @@ module S = FStar.Seq
 
 include Spec.Hash.Lemmas0
 
+open Lib.IntTypes
+
 open Spec.Agile.Hash
 open Spec.Hash.Definitions
 open Spec.Hash.PadFinish
 
 friend Spec.Agile.Hash
+
+let extra_state_add_nat_bound_lem (#a:hash_alg{is_blake a}) (s : extra_state a)
+                                  (n:nat{n <= maxint (extra_state_int_type a)}) :
+  Lemma
+  (requires extra_state_v s + n <= maxint (extra_state_int_type a))
+  (ensures extra_state_v (extra_state_add_nat s n) ==
+             extra_state_v s + n) = ()
+
+let extra_state_add_nat_bound_associative_lem (#a:hash_alg{is_blake a}) (s : extra_state a)
+                                              (n1 n2 : range_t (extra_state_int_type a)) :
+  Lemma
+  (requires n1 + n2 <= maxint (extra_state_int_type a))
+  (ensures
+       (extra_state_add_nat (extra_state_add_nat s n1) n2 ==
+        extra_state_add_nat s (n1 + n2))) =
+  let s1 = extra_state_add_nat s n1 in
+  let s2 = extra_state_add_nat s1 n2 in
+  let s3 = extra_state_add_nat s (n1 + n2) in
+  let s1_v = extra_state_v s1 in
+  let s2_v = extra_state_v s2 in
+  let s3_v = extra_state_v s3 in
+  assert(extra_state_add_nat (extra_state_add_nat s n1) n2 ==
+          (s +. nat_to_extra_state a n1) +. nat_to_extra_state a n2);
+  assert(s1_v == (extra_state_v s + n1) @%. U64);
+  assert(s2_v == s1_v + n2 @%. U64);
+  assert(s2_v == (s1_v + n2) % modulus U64);
+  Math.Lemmas.lemma_mod_add_distr n2 (extra_state_v s + n1) (modulus U64);
+  assert(s2_v == (extra_state_v s + n1 + n2) % modulus U64);
+  Math.Lemmas.lemma_mod_add_distr (extra_state_v s) (n1 + n1) (modulus U64);
+  assert(s3_v == (extra_state_v s + n1 + n2) % modulus U64);
+  assert(s2_v == s3_v)
+
 
 (* Lemmas such as: relationship between maximum lengths, incremental API vs.
  * NIST reference, etc. *)
