specs/Spec.Agile.Hash.fst
@@ -30,14 +30,16 @@ let update a =
       let blake_state, totlen = h in
       // We should never have overflows given the restriction on buffer lengths, so
       // this should be equivalent to a nat addition
-      let totlen = totlen +. u64 (size_block a) in
+//      let totlen = totlen +. u64 (size_block a) in
+      let totlen = extra_state_add_nat totlen (size_block a) in
       (Spec.Blake2.blake2_update_block Spec.Blake2.Blake2S false (v #U64 #SEC totlen) l blake_state,
        totlen)
   | Blake2B -> fun h l ->
       let blake_state, totlen = h in
       // We should never have overflows given the restriction on buffer lengths, so
       // this should be equivalent to a nat addition
-      let totlen = totlen +. u64 (size_block a) in
+//      let totlen = totlen +. u64 (size_block a) in
+      let totlen = extra_state_add_nat totlen (size_block a) in
       (Spec.Blake2.blake2_update_block Spec.Blake2.Blake2B false (v #U64 #SEC totlen) l blake_state,
        totlen)
 
